

$$1) y_1[n] = x[n] \times h[n] \quad -1$$

$$2) y_2[n] = x[n+2] \times h[n]$$

$$3) y_3[n] = x[n] \times h[n+2]$$

$$4) y_1[n] = \sum_{k=-\infty}^{\infty} h[k] x[n-k]$$

$$y_1[n] = h[-1] x[n+1] + h[1] x[n-1]$$

$$\Rightarrow 2x[n+1] + 2x[n-1]$$

$$y_1[n] = 2\delta[n+1] + 4\delta[n-1] + 2\delta[n+1] - 2\delta[n-2]$$

$$y_2[n] = y_1[n+2] \quad y_1[n] = x[n] \times h[n]$$

$$\Rightarrow \sum_{k=-\infty}^{+\infty} x[n] h[n-k]$$

$$y_3[n] = y_1[n+2]$$

$$h[k] = \left(\frac{1}{2}\right)^{k-1} \{a[k+3] - a[k-1]\} \quad (2)$$

$$A = h-9 \quad B = h+3$$

$$a[n] = \left(\frac{1}{2}\right)^n a[1]$$

$$h[h] = a[h] \quad y[n] = a[n] \times h[h]$$

$$\Rightarrow a_1[h-2] \times h[h+2] \Rightarrow \sum_{k=-\infty}^{\infty} a_1[k-2] h_1[h-k+2]$$

$$y[n] = a_1[n] \times a_1[n] \times h_1[n]$$

$$y[n] = 2 \left[1 - \left(\frac{1}{2}\right)^{n+1} \right] a[n]$$

$$y[n] = a[n] \times h[n] = \sum_{k=-\infty}^{+\infty} [k] h[n-k] \quad (4)$$

$$y[n] = a[3] h[n-3] + a[4] h[n-4] + a[5] h[n-5]$$

$$+ a[6] h[n-6] + a[7] h[n-7] + a[8] h[n-8]$$

$$y[n] = \begin{cases} h-6 & 7 \leq h \leq 11 \\ 6 & 12 \leq h \leq 18 \\ 24-h & 19 \leq h \leq 23 \\ 0 & \text{باقي } h \end{cases}$$

$$y[n] = \sum_{k=0}^{\infty} a[k] h[n-k] = \sum_{k=0}^{\infty} h[n-k] \quad (5)$$

$$N=4$$

$$y[n] = a[n] * h[n] = \sum_{k=-\infty}^{+\infty} a[k] h[n-k] \quad (6)$$

$$\Rightarrow \sum_{k=-1}^{\infty} \left(\frac{1}{3}\right)^k u[n+k-1]$$

$$y[n] = \sum_{p=0}^{\infty} \left(\frac{1}{3}\right)^{p+1} u[n+p]$$

$$y[n] = \begin{cases} \frac{3^n}{2} & n > 0 \\ \frac{1}{2} & n \leq 0 \end{cases}$$

$$y[n] = \sum_{k=-\infty}^{\infty} a[k] g[n-2k] \quad (7)$$

$$g[n] = u[n] - u[n-4]$$

$$y[n] = \sum_{k=-\infty}^{+\infty} a[k] g[n-2k] = g[n-4]$$

$$\Rightarrow u[n-4] - u[n-8]$$

$$g(t) \times h(t) = \int_{-\infty}^{+\infty} g(\tau) h(t-\tau) d\tau \quad (8)$$

$$\Rightarrow \int_{-\infty}^{+\infty} h(\tau) g(t-\tau) d\tau$$

$$h(t) = \delta(t+2) + 2\delta(t+1)$$

$$g(t) = \begin{cases} t+3 & -2 < t \leq -1 \\ t+4 & -1 < t \leq 0 \\ 2-2t & 0 < t \leq 1 \\ 0 & \text{otherwise} \end{cases}$$

$$h(\tau) = e^{2\tau} u(-\tau+4) + e^{-\tau} u(\tau-5) \quad (9)$$

$$\Rightarrow \begin{cases} e^{-2\tau} & \tau > 5 \\ e^{2\tau} & \tau > 4 \\ 0 & 4 < \tau < 5 \end{cases}$$

$$h(-\tau) = \begin{cases} e^{2\tau} & \tau > -5 \\ e^{-2\tau} & \tau > -4 \\ 0 & -5 < \tau < -4 \end{cases}$$

$$A = \tau - 5 \quad B = \tau - 4$$

$$y(t) = \begin{cases} t & 0 \leq t \leq a \\ a & a \leq t \leq 1 \\ 1+a-t & 1 \leq t \leq 1+a \\ 0 & \text{دیگر} \end{cases} \quad (1)$$

$$\alpha = 1$$

(11)

$$y(t) = \dots + e^{-(t-6)} u(t+6) + e^{-(t+3)} \dots \quad (12)$$

$$e^{-t}(1 + e^{-3} + e^{-6} + \dots) = e^{-t} \frac{1}{1 - e^{-3}} \quad \Leftarrow 0 \leq t < \frac{3}{1},$$

$$\left(\frac{1}{5}\right)^h u[h] - A \left(\frac{1}{5}\right)^{h-1} u[h-1] = \delta[h] \quad (13)$$

$$A = \frac{1}{3}$$

$$h[n] - \frac{1}{5} h[n-1] = \delta[n]$$

← (13)

$$h[n] \times (\delta[n] - \frac{1}{5} \delta[n-1]) = \delta[n]$$

$$g[n] = \delta[n] - \delta[n] - \frac{1}{2} \delta[n-1]$$

$$\int_{-\infty}^{+\infty} |h_1(\tau)| d\tau = \int_0^{\infty} e^{-\tau} d\tau = 1$$

(14)

$$\int_{-\infty}^{+\infty} |h_2(\tau)| d\tau = \int_0^{\infty} e^{-\tau} |\cos 2t| d\tau$$

ex. 6.8 LTI

(15)